src/Core_Erlang_Semantics.v
@@ -8,32 +8,302 @@ Export Core_Erlang_Environment.Environment.
 
 Import ListNotations.
 
+(** For biuilt-in arithmetic calls *)
+Definition eval_arith (fname : string) (params : list Value) : Value + Exception :=
+match fname, params with
+(** addition *)
+| "+"%string, [VLit (Integer a); VLit (Integer b)] => inl (VLit (Integer (a + b)))
+| "+"%string, [a; b]                               => inr (badarith (VCons a b))
+(** subtraction *)
+| "-"%string, [VLit (Integer a); VLit (Integer b)] => inl (VLit (Integer (a - b)))
+| "-"%string, [a; b]                               => inr (badarith (VCons a b))
+(** anything else *)
+| _         , _                                    => inr (undef (VLit (Atom fname)))
+end.
+
+(** For IO maniputaion: *)
+Definition eval_io (fname : string) (params : list Value) (eff : SideEffectList) 
+   : ((Value + Exception) * SideEffectList) :=
+match fname, length params, params with
+(** writing *)
+| "fwrite"%string, 1, _ => (inl ok                                    , eff ++ [(Output, params)])
+(** reading *)
+| "fread"%string , 2, e => (inl (VTuple [ok; nth 1 params ErrorValue]), eff ++ [(Input, params)])
+(** anything else *)
+| _              , _, _ => (inr (undef (VLit (Atom fname)))           , eff)
+end.
+
+Definition eval_logical (fname : string) (params : list Value) : Value + Exception :=
+match fname, params with
+(** logical and *)
+| "and"%string, [a; b] => 
+   match a, b with
+   | VLit (Atom "true") , VLit (Atom "true")    => inl ttrue
+   | VLit (Atom "false"), VLit (Atom "true")    => inl ffalse
+   | VLit (Atom "true") , VLit (Atom "false")   => inl ffalse
+   | VLit (Atom "false"), VLit (Atom "false")   => inl ffalse
+   | _                         , _              => inr (badarg (VCons a b))
+   end
+(** logical or *)
+| "or"%string, [a; b] =>
+   match a, b with
+   | VLit (Atom "true") , VLit (Atom "true")    => inl ttrue
+   | VLit (Atom "false"), VLit (Atom "true")    => inl ttrue
+   | VLit (Atom "true") , VLit (Atom "false")   => inl ttrue
+   | VLit (Atom "false"), VLit (Atom "false")   => inl ffalse
+   | _                         , _              => inr (badarg (VCons a b))
+   end
+(** logical not *)
+| "not"%string, [a] =>
+   match a with
+   | VLit (Atom "true")  => inl ffalse
+   | VLit (Atom "false") => inl ttrue
+   | _                   => inr (badarg a)
+   end
+(** anything else *)
+| _ , _ => inr (undef (VLit (Atom fname)))
+end.
+
+Definition eval_equality (fname : string) (params : list Value) : Value + Exception :=
+match fname, params with
+| "=="%string,  [v1; v2] (* TODO: with floats, this one should be adjusted *)
+| "=:="%string, [v1; v2] => if bValue_eq_dec v1 v2 then inl ttrue else inl ffalse
+| "/="%string,  [v1; v2] (* TODO: with floats, this one should be adjusted *)
+| "=/="%string, [v1; v2] => if bValue_eq_dec v1 v2 then inl ffalse else inl ttrue
+(** anything else *)
+| _ , _ => inr (undef (VLit (Atom fname)))
+end.
+
+Fixpoint eval_append (v1 v2 : Value) : Value + Exception :=
+match v1, v2 with
+| VNil, VNil => inl VNil
+| VNil, VCons x y => inl (VCons x y)
+| VCons x y, VNil => inl (VCons x y)
+| VCons x y, VCons x' y' =>
+  match y with
+  | VCons z w => match eval_append y (VCons x' y') with
+                 | inr ex => inr ex
+                 | inl res => inl (VCons x res)
+                 end
+  | VNil      => inl (VCons x (VCons x' y'))
+  | z         => inl (VCons x (VCons y (VCons x' y')))
+  end
+| _, _ => inr (badarg (VCons v1 v2))
+end.
+
+Fixpoint subtract_elem (v1 v2 : Value) : Value :=
+match v1 with
+| VNil => VNil
+| VCons x y =>
+  match y with
+  | VNil => if bValue_eq_dec x v2 then VNil else VCons x y
+  | VCons z w => if bValue_eq_dec x v2 then y else VCons x y
+  | z => if bValue_eq_dec x v2 then VCons z VNil else if bValue_eq_dec z v2 then VCons x VNil else VCons x y
+  end
+| _ => ErrorValue
+end.
+
+Fixpoint eval_subtract (v1 v2 : Value) : Value + Exception :=
+match v1, v2 with
+| VNil, VNil => inl VNil
+| VNil, VCons x y => inl VNil
+| VCons x y, VNil => inl (VCons x y)
+| VCons x y, VCons x' y' => 
+   match y' with
+   | VNil => inl (subtract_elem (VCons x y) x')
+   | VCons z w => eval_subtract (subtract_elem (VCons x y) x') y'
+   | z => inl (subtract_elem (subtract_elem (VCons x y) x') z)
+   end
+| _        , _         => inr (badarg (VCons v1 v2))
+end.
+
+Definition eval_transform_list (fname : string) (params : list Value) : Value + Exception :=
+match fname, params with
+| "++"%string, [v1; v2] => eval_append v1 v2
+| "--"%string, [v1; v2] => eval_subtract v1 v2
+| _ , _ => inr (undef (VLit (Atom fname)))
+end.
+
+Fixpoint transform_tuple (v : Value) : Value + Exception :=
+match v with
+| VTuple l => inl ((fix unfold_list l :=
+                   match l with
+                   | [] => VNil
+                   | x::xs => VCons x (unfold_list xs)
+                   end) l)
+| _        => inr (badarg v)
+end.
+
+Fixpoint transform_list (v : Value) : list Value + Exception :=
+match v with
+| VNil      => inl []
+| VCons x y => match y with
+               | VNil => inl [x]
+               | VCons z w => match (transform_list y) with
+                              | inr ex => inr ex
+                              | inl res => inl (x::res)
+                              end
+               | z => inl [x; z]
+               end
+| _         => inr (badarg v)
+end.
+
+Definition eval_list_tuple (fname : string) (params : list Value) : Value + Exception :=
+match fname, params with
+| "tuple_to_list"%string, [v] => transform_tuple v
+| "list_to_tuple"%string, [v] => match (transform_list v) with
+                                 | inr ex => inr ex
+                                 | inl l => inl (VTuple l)
+                                 end
+| _                     , _   => inr (undef (VLit (Atom fname)))
+end.
+
+Definition eval_cmp (fname : string) (params : list Value) : Value + Exception :=
+match fname, params with
+| "<"%string,  [v1; v2] => if value_less v1 v2 then inl ttrue else inl ffalse
+| "<="%string, [v1; v2] => if orb (value_less v1 v2) (bValue_eq_dec v1 v2) 
+                           then inl ttrue else inl ffalse
+| ">"%string,  [v1; v2] => if value_less v2 v1 then inl ttrue else inl ffalse
+| ">="%string, [v1; v2] => if orb (value_less v2 v1) (bValue_eq_dec v1 v2) 
+                           then inl ttrue else inl ffalse
+(** anything else *)
+| _ , _ => inr (undef (VLit (Atom fname)))
+end.
+
 (* TODO: Always can be extended, this function simulates inter-module calls *)
 Definition eval (fname : string) (params : list Value) (eff : SideEffectList) 
    : ((Value + Exception) * SideEffectList) :=
-match fname, length params, params with
-(** addition *)
-| "plus"%string, 2, [VLit (Integer a); VLit (Integer b)] => 
-     (inl (VLit (Integer (a + b))), eff)
-(** faulty addition *)
-| "plus"%string, 2, [a; b] => (inr (badarith (VCons a b)), eff)
-(** writing *)
-| "fwrite"%string, _, _ => (inl ok, eff ++ [(Output, params)])
-(** reading *)
-| "fread"%string, 2, e => (inl (VTuple [ok; nth 1 params ErrorValue]), eff ++ [(Input, params)])
-
-(** and operator *)
-| "and"%string, 2, [VLit (Atom a); VLit (Atom b)] => 
-   match a, b with
-   | "true"%string, "true"%string => (inl ttrue, eff)
-   | "false"%string, "true"%string => (inl ffalse, eff)
-   | "true"%string, "false"%string => (inl ffalse, eff)
-   | "false"%string, "false"%string => (inl ffalse, eff)
-   | _, _ => (inr (badarg (VCons (VLit (Atom a)) (VLit (Atom b)))), eff)
-   end
+match fname with
+| "+"%string      | "-"%string     => (eval_arith fname params, eff)
+| "fwrite"%string | "fread"%string => eval_io fname params eff
+| "and"%string    | "or"%string
+| "not"%string                     => (eval_logical fname params, eff)
+| "=="%string     | "=:="%string
+| "/="%string     | "=/="%string   => (eval_equality fname params, eff)
+| "++"%string     | "--"%string    => (eval_transform_list fname params, eff)
+| "tuple_to_list"%string
+| "list_to_tuple"%string           => (eval_list_tuple fname params, eff)
+| "<"%string      | ">"%string 
+| "<="%string     | ">="%string    => (eval_cmp fname params, eff)
 (** anything else *)
-| _, _, _ => (inr (undef (VLit (Atom fname))), eff)
+| _                                => (inr (undef (VLit (Atom fname))), eff)
 end.
+
+(** Tests *)
+
+Compute (eval "+" [VLit (Integer 1); VLit (Integer 2)]) [] = (inl (VLit (Integer 3)), []).
+Compute (eval "-" [VLit (Integer 1); VLit (Integer 2)]) [] = (inl (VLit (Integer (-1))), []).
+Compute (eval "+" [VLit (Atom "foo"); VLit (Integer 2)]) [] 
+    = (inr (badarith (VCons (VLit (Atom "foo")) (VLit (Integer 2)))), []).
+Compute (eval "+" [VLit (Integer 1); VLit (Atom "foo")]) [] 
+    = (inr (badarith (VCons (VLit (Integer 2)) (VLit (Atom "foo")))), []).
+Compute (eval "-" [VLit (Atom "foo"); VLit (Integer 2)]) [] 
+    = (inr (badarith (VCons (VLit (Atom "foo")) (VLit (Integer 2)))), []).
+Compute (eval "-" [VLit (Integer 1); VLit (Atom "foo")]) [] 
+    = (inr (badarith (VCons (VLit (Integer 2)) (VLit (Atom "foo")))), []).
+Compute (eval "-" [VLit (Atom "foo")]) [] 
+    = (inr (undef (VLit (Atom "-"))), []).
+Compute (eval "+" [VLit (Atom "foo")]) [] 
+    = (inr (undef (VLit (Atom "+"))), []).
+
+Compute (eval "not" [ttrue]) [] = (inl ffalse, []).
+Compute (eval "not" [ffalse]) [] = (inl ttrue, []).
+Compute (eval "not" [VLit (Integer 5)]) [] = (inr (badarg (VLit (Integer 5))), []).
+Compute (eval "not" [VLit (Integer 5); VEmptyTuple]) [] = (inr (undef (VLit (Atom "not"))), []).
+
+Compute (eval "and" [ttrue; ttrue]) [] = (inl ttrue, []).
+Compute (eval "and" [ttrue; ffalse]) [] = (inl ffalse, []).
+Compute (eval "and" [ffalse; ttrue]) [] = (inl ffalse, []).
+Compute (eval "and" [ffalse; ffalse]) [] = (inl ffalse, []).
+Compute (eval "and" [ttrue; VEmptyTuple]) [] = (inr (badarg (VCons (VLit (Atom "true")) (VTuple []))), []).
+Compute (eval "and" [ttrue]) [] = (inr (undef (VLit (Atom "and"))), []).
+
+Compute (eval "or" [ttrue; ttrue]) [] = (inl ttrue, []).
+Compute (eval "or" [ttrue; ffalse]) [] = (inl ttrue, []).
+Compute (eval "or" [ffalse; ttrue]) [] = (inl ttrue, []).
+Compute (eval "or" [ffalse; ffalse]) [] = (inl ffalse, []).
+Compute (eval "or" [ttrue; VEmptyTuple]) [] = (inr (badarg (VCons (VLit (Atom "true")) (VTuple []))), []).
+Compute (eval "or" [ttrue]) [] = (inr (undef (VLit (Atom "or"))), []).
+
+Compute (eval "fwrite" [ttrue]) [] = (inl ok, [(Output, [ttrue])]).
+Compute (eval "fwrite" [VMap [(ttrue, ttrue)]]) [] = (inl ok, [(Output, [VMap [(ttrue, ttrue)]])]).
+Compute (eval "fwrite" []) [] = (inr (undef (VLit (Atom "fwrite"))), []).
+
+Compute (eval "fread" [VLit (Atom "foo.txt"); ttrue]) [] = 
+   (inl (VTuple [ok; ttrue]), [(Input, [VLit (Atom "foo.txt"); ttrue])]).
+Compute (eval "fread" [VLit (Atom "foo.txt"); VMap [(ttrue, ttrue)]]) [] = 
+   (inl (VTuple [ok; VMap [(ttrue, ttrue)]]), [(Input, [VLit (Atom "foo.txt"); VMap [(ttrue, ttrue)]])]).
+Compute (eval "fread" []) [] = (inr (undef (VLit (Atom "fread"))), []).
+
+Compute (eval "==" [ttrue; ttrue]) [] = (inl ttrue, []).
+Compute (eval "==" [ttrue; ffalse]) [] = (inl ffalse, []).
+Compute (eval "==" [VClos [] [] 1 [] EEmptyMap; ttrue]) [] = (inl ffalse, []).
+Compute (eval "==" [VClos [] [] 1 [] EEmptyMap; VClos [] [] 2 [] EEmptyMap]) [] = (inl ffalse, []).
+Compute (eval "==" [VClos [] [] 1 [] EEmptyMap; VClos [] [] 1 [] EEmptyMap]) [] = (inl ttrue, []).
+
+Compute (eval "/=" [ttrue; ttrue]) [] = (inl ffalse, []).
+Compute (eval "/=" [ttrue; ffalse]) [] = (inl ttrue, []).
+Compute (eval "/=" [VClos [] [] 1 [] EEmptyMap; ttrue]) [] = (inl ttrue, []).
+Compute (eval "/=" [VClos [] [] 1 [] EEmptyMap; VClos [] [] 2 [] EEmptyMap]) [] = (inl ttrue, []).
+Compute (eval "/=" [VClos [] [] 1 [] EEmptyMap; VClos [] [] 1 [] EEmptyMap]) [] = (inl ffalse, []).
+Compute (eval "/=" [ttrue]) [] = (inr (undef (VLit (Atom "/="))), []).
+
+Definition l1 : Value := VCons ttrue VNil.
+Definition l2 : Value := VCons ttrue ttrue.
+Definition l3 : Value := VCons (VCons ttrue ttrue) ttrue.
+Definition l4 : Value := VCons ttrue (VCons ttrue (VCons ttrue VNil)).
+Definition l5 : Value := VCons ttrue (VCons ttrue ttrue).
+
+Compute (eval "++" [ttrue; ttrue]) [] = (inr (badarg _), []).
+Compute (eval "++" [l1; l1]) [].
+Compute (eval "++" [l1; l2]) [].
+Compute (eval "++" [l1; l3]) [].
+Compute (eval "++" [l3; l3]) [].
+
+Compute (eval "--" [ttrue; ttrue]) [] = (inr (badarg _), []).
+Compute (eval "--" [l1; l1]) [].
+Compute (eval "--" [l1; l2]) [].
+Compute (eval "--" [l1; l3]) [].
+Compute (eval "--" [l3; l3]) [].
+Compute (eval "--" [l3; l1]) [].
+
+Compute (eval "tuple_to_list" [VTuple [ttrue; ttrue; ttrue; l1]] []).
+Compute (eval "tuple_to_list" [VTuple [ttrue; ttrue; l5; l1]] []).
+Compute (eval "tuple_to_list" [VTuple [ttrue; l3; ttrue; l1]] []).
+Compute (eval "tuple_to_list" [VTuple [ttrue; ttrue; l2; l1]] []).
+Compute (eval "tuple_to_list" [ttrue] []).
+
+Compute (eval "list_to_tuple" [l1] []).
+Compute (eval "list_to_tuple" [l2] []).
+Compute (eval "list_to_tuple" [l3] []).
+Compute (eval "list_to_tuple" [l4] []).
+Compute (eval "list_to_tuple" [l5] []).
+
+Compute (eval "<" [ttrue; ttrue]) [] = (inl ffalse, []).
+Compute (eval "<" [ttrue; ffalse]) [] = (inl ffalse, []).
+Compute (eval "<" [VClos [] [] 1 [] EEmptyMap; VEmptyMap]) [] = (inl ttrue, []).
+Compute (eval "<" [VClos [] [] 1 [] EEmptyMap; VClos [] [] 2 [] EEmptyMap]) [] = (inl ttrue, []).
+Compute (eval "<" [VClos [] [] 1 [] EEmptyMap; VClos [] [] 1 [] EEmptyMap]) [] = (inl ffalse, []).
+
+Compute (eval "<=" [ttrue; ttrue]) [] = (inl ttrue, []).
+Compute (eval "<=" [ttrue; ffalse]) [] = (inl ffalse, []).
+Compute (eval "<=" [VClos [] [] 1 [] EEmptyMap; VEmptyMap]) [] = (inl ttrue, []).
+Compute (eval "<=" [VClos [] [] 1 [] EEmptyMap; VClos [] [] 2 [] EEmptyMap]) [] = (inl ttrue, []).
+Compute (eval "<=" [VClos [] [] 1 [] EEmptyMap; VClos [] [] 1 [] EEmptyMap]) [] = (inl ttrue, []).
+
+Compute (eval ">" [ttrue; ttrue]) [] = (inl ffalse, []).
+Compute (eval ">" [ffalse; ttrue]) [] = (inl ffalse, []).
+Compute (eval ">" [VEmptyMap; VClos [] [] 1 [] EEmptyMap]) [] = (inl ttrue, []).
+Compute (eval ">" [VClos [] [] 2 [] EEmptyMap; VClos [] [] 1 [] EEmptyMap]) [] = (inl ttrue, []).
+Compute (eval ">" [VClos [] [] 1 [] EEmptyMap; VClos [] [] 1 [] EEmptyMap]) [] = (inl ffalse, []).
+
+Compute (eval ">=" [ttrue; ttrue]) [] = (inl ttrue, []).
+Compute (eval ">=" [ffalse; ttrue]) [] = (inl ffalse, []).
+Compute (eval ">=" [VEmptyMap; VClos [] [] 1 [] EEmptyMap]) [] = (inl ttrue, []).
+Compute (eval ">=" [VClos [] [] 2 [] EEmptyMap; VClos [] [] 1 [] EEmptyMap]) [] = (inl ttrue, []).
+Compute (eval ">=" [VClos [] [] 1 [] EEmptyMap; VClos [] [] 1 [] EEmptyMap]) [] = (inl ttrue, []).
+
+(** End of tests *)
 
 Reserved Notation "| env , id , e , eff | -e> | id' , e' , eff' |" (at level 70).
 Inductive eval_expr : Environment -> nat -> Expression -> SideEffectList -> nat ->
